Have a general kv_replica_main parameterized over filename and hostname

external/Goose/github_com/mit_pdos/gokv/simplepb/apps/closed.v
@@ -19,16 +19,9 @@ Definition config_main: val :=
     config.Server__Serve (config.MakeServer (![slice.T uint64T] "servers")) configHost;;
     #().
 
-Definition kv_replica_main1: val :=
-  rec: "kv_replica_main1" <> :=
+Definition kv_replica_main: val :=
+  rec: "kv_replica_main" "fname" "me" :=
     let: "x" := ref (zero_val uint64T) in
     "x" <-[uint64T] #1;;
-    kv64.Start #(str"kv.data") r1;;
-    #().
-
-Definition kv_replica_main2: val :=
-  rec: "kv_replica_main2" <> :=
-    let: "x" := ref (zero_val uint64T) in
-    "x" <-[uint64T] #1;;
-    kv64.Start #(str"kv.data") r2;;
+    kv64.Start "fname" "me";;
     #().
