src/program_proof/simplepb/apps/closed_wpcs.v
@@ -17,14 +17,12 @@ Section closed_wpcs.
 Context `{!heapGS Σ}.
 Context `{!kv64G Σ}.
 
-Definition replica_fname := "kv.data".
-
-Lemma wpc_kv_replica_main1 γsys γsrv Φc:
-  ((∃ data' : list u8, replica_fname f↦data' ∗ ▷ file_crash (own_Server_ghost γsys γsrv) data') -∗
+Lemma wpc_kv_replica_main γsys γsrv Φc fname me :
+  ((∃ data' : list u8, fname f↦data' ∗ ▷ file_crash (own_Server_ghost γsys γsrv) data') -∗
     Φc) -∗
-  is_pb_host 1%Z γsys γsrv -∗ sys_inv γsys -∗
-  (∃ data : list u8, replica_fname f↦data ∗ file_crash (own_Server_ghost γsys γsrv) data) -∗
-  WPC kv_replica_main1 #() @ ⊤
+  is_pb_host me γsys γsrv -∗ sys_inv γsys -∗
+  (∃ data : list u8, fname f↦data ∗ file_crash (own_Server_ghost γsys γsrv) data) -∗
+  WPC kv_replica_main #(LitString fname) #me @ ⊤
   {{ _, True }}
   {{ Φc }}
 .
@@ -32,7 +30,7 @@ Proof.
   iIntros "HΦc #Hpbhost #Hsys Hpre".
   iDestruct "Hpre" as (?) "[Hfile Hcrash]".
 
-  unfold kv_replica_main1.
+  unfold kv_replica_main.
   wpc_call.
   { iApply "HΦc". iExists _. iFrame. }
 
@@ -59,72 +57,7 @@ Proof.
   { iAccu. }
   {
     iModIntro.
-    instantiate (1:=(|C={⊤}=> ∃ data', replica_fname f↦ data' ∗ ▷ file_crash (own_Server_ghost γsys γsrv) data')).
-    iIntros "[H1 H2]".
-    iModIntro.
-    iExists _.
-    iFrame.
-  }
-  iIntros "Hfile_ctx".
-  wpc_apply (wpc_crash_mono _ _ _ _ _ (True%I) with "[HΦc]").
-  { iIntros "_".
-    iIntros "H".
-    iMod "H".
-    iModIntro.
-    iApply "HΦc".
-    done. }
-  iApply wp_wpc.
-  wp_pures.
-
-  wp_apply (wp_Start with "[Hfile_ctx]").
-  {
-    iFrame "∗#".
-  }
-  wp_pures.
-  done.
-Qed.
-
-Lemma wpc_kv_replica_main2 γsys γsrv Φc:
-  ((∃ data' : list u8, replica_fname f↦data' ∗ ▷ file_crash (own_Server_ghost γsys γsrv) data') -∗
-    Φc) -∗
-  is_pb_host 2%Z γsys γsrv -∗ sys_inv γsys -∗
-  (∃ data : list u8, replica_fname f↦data ∗ file_crash (own_Server_ghost γsys γsrv) data) -∗
-  WPC kv_replica_main2 #() @ ⊤
-  {{ _, True }}
-  {{ Φc }}
-.
-Proof.
-  iIntros "HΦc #Hpbhost #Hsys Hpre".
-  iDestruct "Hpre" as (?) "[Hfile Hcrash]".
-
-  unfold kv_replica_main1.
-  wpc_call.
-  { iApply "HΦc". iExists _. iFrame. }
-
-  iCache with "HΦc Hfile Hcrash".
-  { iApply "HΦc". iExists _. iFrame. }
-  wpc_bind (Primitive2 _ _ _).
-  wpc_frame.
-  iApply wp_crash_borrow_generate_pre.
-  { done. }
-  wp_apply (wp_ref_of_zero).
-  { done. }
-  iIntros (?) "Hl".
-  iIntros "Hpreborrow".
-  iNamed 1.
-  wpc_pures.
-  wpc_bind (store_ty _ _).
-  wpc_frame.
-  wp_store.
-  iModIntro.
-  iNamed 1.
-
-  iApply wpc_cfupd.
-  wpc_apply (wpc_crash_borrow_inits with "Hpreborrow [Hfile Hcrash] []").
-  { iAccu. }
-  {
-    iModIntro.
-    instantiate (1:=(|C={⊤}=> ∃ data', replica_fname f↦ data' ∗ ▷ file_crash (own_Server_ghost γsys γsrv) data')).
+    instantiate (1:=(|C={⊤}=> ∃ data', fname f↦ data' ∗ ▷ file_crash (own_Server_ghost γsys γsrv) data')).
     iIntros "[H1 H2]".
     iModIntro.
     iExists _.
